---
title: "T1W6L2: completing the square"
---
#methods #AE #lesson
# completing the square
i studied jap instead so ill do this later lol :(
future thomas here, did it later

# recap
| Names                          | Equation Form   |
| ------------------------------ | --------------- |
| general or y-intercept form    | $y=ax^2+bx+c$   |
| factorised or x-intercept form | $y=a(x-p)(x-q)$ |
| square or turning point form   | $y=a(x-h)^2+k$                |
various features can be quickly identified from each of these forms, and used to sketch a graph.

# completing the square
- completing the square is useful for converting quadratics into turning point form in order to graph or solve them.
- Remember, perfect squares factorise as follows:
$$x^2+2nx+n^2=(x+n)^2$$
- 2nx is x coefficient, n^2 is square of half the coefficient, and n is half the coefficient. 
- To complete the square, it is faster to use it in the following form: $$x^2+2nx=(x+n)^2-n^2$$
- example
	- consider $2x^2+6x+1$
		1. factorise out the 2 from the first two terms: $$2(x^2+3x)+1$$
		2. halve the 3, then square it: $3\div2=\frac{3}{2}$, $\left( \frac{3}{2} \right)^2=\frac{9}{4}$
		3. form the perfect square $x^2+3x=\left( x+\frac{3}{2} \right)^2-\frac{9}{4}$
		4. rewrite $2(x^2+3x)+1:2\left( \left( x+\frac{3}{2} \right)^2 -\frac{9}{4} \right)+1$
		5. expand and simplify $2\left( x+\frac{3}{2} \right)^2-\frac{7}{2}$

$x^2 + 2nx = (2+x)^2 - n^2$
no longer have to explicitly create a perfect square.
the new process more simple and streamlined, but if you're still confused, you can use the old way.
solve $2x^2-3x-1=0$ by completing the square
$2\left( x^2-\frac{3}{2}x \right)-1$
$x^2-\frac{3}{2}x=(x+\frac{3}{4})^2-\frac{9}{16}$
$=2\left( x+\frac{3}{4} \right)^2-\frac{9}{16}+\frac{16}{16}$
$=2\left( x+\frac{3}{4} \right)^2+\frac{7}{16}$